theories/L2_typeStripped/compile.v
@@ -34,10 +34,10 @@ Inductive Term : Type :=
 | TConstruct : inductive -> nat (* cnstr no *) ->
                nat (* # pars *) -> nat (* # args *) -> Term
                                   (* use Defs to code branches *)
-| TCase      : (inductive * nat) (* # of pars *) ->
+| TCase      : nat (* # of pars *) ->
                Term (* discriminee *) -> Brs (* # args, branch *) -> Term
 | TFix       : Defs -> nat -> Term
-| TWrong     : Term
+| TWrong     : string -> Term
 with Terms : Type :=
 | tnil : Terms
 | tcons : Term -> Terms -> Terms
@@ -80,9 +80,9 @@ Function strip (t:L1gTerm) : Term :=
     | L1g.compile.TConst nm => TConst nm
     | L1g.compile.TInd i => TInd i
     | L1g.compile.TConstruct i m np na => TConstruct i m np na
-    | L1g.compile.TCase n _ mch brs => TCase n (strip mch) (stripBs brs)
+    | L1g.compile.TCase n _ mch brs => TCase (snd n) (strip mch) (stripBs brs)
     | L1g.compile.TFix ds n => TFix (stripDs ds) n
-    | L1g.compile.TWrong _ => TWrong
+    | L1g.compile.TWrong str => TWrong str
   end
 with strips (ts:L1gTerms) : Terms := 
   match ts with
